another big refactor

Diploma/Order/MonomialOrder.lean
@@ -11,62 +11,48 @@ namespace algebra
 
 class MonomialOrder (α : Type u) [HMul α α α] extends LinearOrder α := 
  add_le_add : ∀ a b c: α, a < b → a * c < b * c
-      
-section monomials_lex_order
 
-private def Order.blt_lex_impl (v₁ v₂ : Vector Nat n): Bool :=
-  match v₁, v₂ with
-    | ⟨[], _⟩  , ⟨[], _⟩   => true
-    | ⟨x::_, _⟩, ⟨y::_, _⟩ => if x == y then blt_lex_impl v₁.tail v₂.tail 
-                              else x < y
-
+--# Lex order
+--# a <_lex b ↔ ∃ c: a = c ++ p₁, b = c ++ p₂ ∧ p₁[0] < p₂[0]
 def Order.lex_impl (v₁ v₂ : Vector Nat n): Prop :=
   match v₁, v₂ with
-    | ⟨[], _⟩  , ⟨[], _⟩   => True
+    | ⟨[], _⟩  , ⟨[], _⟩   => False
     | ⟨x::_, _⟩, ⟨y::_, _⟩ => if x = y then lex_impl v₁.tail v₂.tail 
                               else x < y
 
 def Order.lex (v₁ v₂ : Variables n order.Lex): Prop := Order.lex_impl v₁ v₂
 
-def Order.lex_le (v₁ v₂ : Variables n order.Lex): Prop := v₁ = v₂ ∨ Order.lex v₁ v₂  
+def Order.lex_le (v₁ v₂ : Variables n order.Lex): Prop := if v₁ = v₂ then True
+                                                          else Order.lex v₁ v₂  
 
-theorem lex_lt_refl : ∀ (a : Variables n order.Lex), Order.lex a a := by
+private def Order.blt_lex_impl (v₁ v₂ : Vector Nat n): Bool :=
+  match v₁, v₂ with
+    | ⟨[], _⟩  , ⟨[], _⟩   => false
+    | ⟨x::_, _⟩, ⟨y::_, _⟩ => if x == y then blt_lex_impl v₁.tail v₂.tail 
+                              else x < y
+
+private def Order.ble_lex_impl (v₁ v₂ : Vector Nat n): Bool := v₁ == v₂ ∨ Order.blt_lex_impl v₁ v₂  
+
+--# Ordering theorems
+theorem lex_le_refl : ∀ (a : Variables n order.Lex), Order.lex_le a a := by
   intro a
-  let rec aux (m: Nat) (v: Variables m order.Lex) : Order.lex_impl v v := by 
-    match v with 
-      | ⟨[], p⟩    => rw [Order.lex_impl]
-                      split
-                      simp at *
-                      simp at p
-                      simp at *                                   
-      | ⟨x::xs, _⟩ => rw [Order.lex_impl]
-                      split
-                      simp
-                      simp at *
-                      simp at *
-                      simp [Nat.le_refl]
-                      rename_i x₁ _ x₂ _ h₁ h₂
-                      have h₃ := Eq.symm h₁.left
-                      have h₄ := Eq.symm h₂.left
-                      rw [h₃, h₄]
-                      simp [Nat.le_refl]
-                      apply aux (m-1) (tail ⟨x::xs, _⟩)
-  exact aux n a
+  match a with 
+    | ⟨[], p⟩    => rw [Order.lex_le]
+                    simp                          
+    | ⟨x::xs, _⟩ => rw [Order.lex_le, Order.lex, Order.lex_impl]
+                    split
+                    simp
+                    simp at *
 
-theorem lex_le_refl : ∀ (a : Variables n order.Lex), Order.lex_le a a := by 
-  intros a
-  rw [Order.lex_le]
-  simp
-
-theorem lex_lt_trans : ∀ (a b c : Variables n order.Lex), Order.lex a b → Order.lex b c → Order.lex a c := by
-  intros v₁ v₂ v₃ h₁ h₂
+theorem lex_lt_trans (a b c : Variables n order.Lex): Order.lex a b → Order.lex b c → Order.lex a c := by
+  intros h₁ h₂
   let rec aux (m: Nat) (a b c: Variables m order.Lex) 
               (ab : Order.lex_impl a b) (bc : Order.lex_impl b c) : Order.lex_impl a c := by 
     match a, b, c with
-      | ⟨[], p⟩,    ⟨[], q⟩,    ⟨[], l⟩    => rw [Order.lex_impl]
-                                              split
-                                              simp
-                                              simp at *
+      | ⟨[], p⟩,    ⟨[], q⟩,    ⟨[], l⟩    => rw [Order.lex_impl] at ab bc
+                                              split at ab 
+                                              split at bc
+                                              repeat contradiction
       | ⟨x::xs, p⟩, ⟨y::ys, q⟩, ⟨z::zs, l⟩ => rw [Order.lex_impl] 
                                               rw [Order.lex_impl] at ab bc
                                               split at ab
@@ -162,34 +148,39 @@ theorem lex_lt_trans : ∀ (a b c : Variables n order.Lex), Order.lex a b → Or
                                               rw [x_cross_eq_x, y_cross_eq_x] at neq₃ bc
                                               have le_le := Nat.lt_trans ab bc
                                               exact le_le                        
-  exact aux n v₁ v₂ v₃ h₁ h₂
+  exact aux n a b c h₁ h₂
 
 theorem lex_le_trans : ∀ (a b c : Variables n order.Lex), Order.lex_le a b → Order.lex_le b c → Order.lex_le a c := 
   by
     intros a b c ab bc
     rw [Order.lex_le]
     rw [Order.lex_le] at ab bc
-    cases ab
-    cases bc
+    split at ab
+    split at bc
     rename_i eq₁ eq₂
     rw [eq₂] at eq₁
     simp [eq₁]
     rename_i eq leq
     rw [←eq] at leq
     simp [leq]
-    cases bc
-    rename_i leq eq
-    rw [eq] at leq
-    simp [leq]
-    apply Or.inr
-    rename_i leq₁ leq₂
-    exact lex_lt_trans a b c leq₁ leq₂ 
+    rw [←eq] at bc
+    exact bc
+    split at bc
+    rename_i neq eq
+    rw [eq] at neq
+    split
+    simp
+    rw [eq] at ab
+    exact ab
+    split
+    simp
+    exact lex_lt_trans a b c ab bc 
 
 theorem lex_lt_antisymm : ∀ (a b : Variables n order.Lex), Order.lex a b → Order.lex b a → a = b := by
   intros v₁ v₂ h₁ h₂
   let rec aux (m: Nat) (a b: Vector Nat m) (ab: Order.lex_impl a b) (ba: Order.lex_impl b a): a = b := by 
     match a, b with
-      | ⟨[], p⟩, ⟨[], q⟩       => simp 
+      | ⟨[], p⟩, ⟨[], _⟩       => simp 
       | ⟨x::xs, p⟩, ⟨y::ys, q⟩ => rw [Order.lex_impl] at ab ba
                                   simp at *
                                   split at ab
@@ -216,66 +207,77 @@ theorem lex_lt_antisymm : ∀ (a b : Variables n order.Lex), Order.lex a b → O
 theorem lex_le_antisymm : ∀ (a b : Variables n order.Lex), Order.lex_le a b → Order.lex_le b a → a = b := by
   intros a b le₁ le₂
   rw [Order.lex_le] at le₁ le₂
-  cases le₁
-  cases le₂
+  split at le₁
+  split at le₂
   rename_i h
   rw [h] 
   rename_i h _
   exact h
-  cases le₂
+  split at le₂
   rename_i h
   simp [h]
-  rename_i h₁ h₂
-  exact lex_lt_antisymm a b h₁ h₂  
+  exact lex_lt_antisymm a b le₁ le₂  
 
-theorem lex_lt_total : ∀ (a b : Variables n order.Lex), Order.lex a b ∨ Order.lex b a := by
-  intros v₁ v₂
-  let rec aux (m: Nat) (a b: Vector Nat m) : Order.lex_impl a b ∨ Order.lex_impl b a := by
+theorem vectors_neq_r_head_neq (v₁ v₂: Vector Nat (Nat.succ n)) (h: v₁ ≠ v₂): head v₁ ≠ head v₂ := by sorry 
+
+theorem lex_lt_semi_total (v₁ v₂ : Variables n order.Lex) (not_eq: v₁ ≠ v₂): Order.lex v₁ v₂ ∨ Order.lex v₂ v₁ := by
+  let rec aux (m: Nat) (a b: Vector Nat m) (not_eq_: a ≠ b): (Order.lex_impl a b ∨ Order.lex_impl b a) := by
     match a, b with
-      | ⟨[], p⟩, ⟨[], q⟩       => rw [Order.lex_impl]
-                                  split
-                                  simp
-                                  simp at *
+      | ⟨[], p⟩, ⟨[], q⟩       => simp at not_eq_
       | ⟨x::xs, p⟩, ⟨y::ys, q⟩ => rw [Order.lex_impl]
-                                  simp [Or.comm]
+                                  split
                                   rw [Order.lex_impl]
                                   split
                                   simp
-                                  split
-                                  split
-                                  simp [Or.comm]
-                                  apply aux (m-1) (tail ⟨x::xs, p⟩) (tail ⟨y::ys, q⟩)
                                   simp at *
-                                  rename_i eq neq heq₁ heq₂
-                                  have s_eq := Eq.symm eq
-                                  have eq_1 := Eq.symm heq₁.left
-                                  have eq_2 := Eq.symm heq₂.left
-                                  rw [eq_1, eq_2] at s_eq
-                                  contradiction
                                   split
                                   simp at *
-                                  rename_i neq eq heq₁ heq₂
-                                  have s_eq := Eq.symm eq
-                                  have eq_1 := heq₁.left
-                                  have eq_2 := heq₂.left
-                                  rw [eq_1, eq_2] at s_eq
-                                  contradiction
                                   simp at *
-                                  rename_i r _ heq₁ heq₂
-                                  have eq_1 := heq₁.left
-                                  have eq_2 := heq₂.left
-                                  rw [eq_1, eq_2]
-                                  simp [Nat.le_total]
-                                  exact r
-  exact aux n v₁ v₂
-
+                                  split
+                                  simp at *
+                                  rename_i eq ceq₁ ceq₂
+                                  have eq₁ := ceq₁.left
+                                  have eq₂ := ceq₂.left
+                                  rw [← eq₁, ←eq₂] at eq
+                                  sorry
+                                  sorry
+                                  -- rename_i eq neq heq₁ heq₂
+                                  -- have s_eq := Eq.symm eq
+                                  -- have eq_1 := Eq.symm heq₁.left
+                                  -- have eq_2 := Eq.symm heq₂.left
+                                  -- rw [eq_1, eq_2] at s_eq
+                                  -- contradiction
+                                  -- split
+                                  -- simp at *
+                                  -- rename_i neq eq heq₁ heq₂
+                                  -- have s_eq := Eq.symm eq
+                                  -- have eq_1 := heq₁.left
+                                  -- have eq_2 := heq₂.left
+                                  -- rw [eq_1, eq_2] at s_eq
+                                  -- contradiction
+                                  -- simp at *
+                                  -- rename_i r _ heq₁ heq₂
+                                  -- have eq_1 := heq₁.left
+                                  -- have eq_2 := heq₂.left
+                                  -- rw [eq_1, eq_2]
+                                  -- simp [Nat.le_total]
+                                  -- exact r
+  exact aux n v₁ v₂ not_eq
+  
 theorem lex_le_total : ∀ (a b : Variables n order.Lex), Order.lex_le a b ∨ Order.lex_le b a := by 
   intros a b
   rw [Order.lex_le, Order.lex_le]
+  split
+  split
+  simp; simp
+  split
   simp
-  rw [or_or_or_comm]
-  simp [lex_lt_total]
+  rename_i h _
+  simp [lex_lt_semi_total, h] 
 
+theorem lex_lt_iff_le_not_le: ∀ (a b : Variables n order.Lex), Order.lex a b ↔ Order.lex_le a b ∧ ¬ Order.lex_le b a := by
+  sorry
+  
 theorem lex_add_lt_add : ∀ a b c: Variables n order.Lex, Order.lex a b → Order.lex (Variables.mul a c) (Variables.mul b c) := by
   intros v₁ v₂ v₃
   let rec aux (m: Nat) (a b c: Variables m order.Lex) : Order.lex_impl a b → Order.lex_impl (Variables.mul a c) (Variables.mul b c) := by
@@ -284,62 +286,83 @@ theorem lex_add_lt_add : ∀ a b c: Variables n order.Lex, Order.lex a b → Ord
     | ⟨[], _⟩, ⟨[], _⟩, ⟨[], _⟩          => rw [Order.lex_impl]
                                             split
                                             simp
-                                            split
+                                            sorry
+                                            sorry
                                             repeat (rename_i prop₁ _ _ _ _ _ _ _ _ _ prop₄ _ _ _
                                                     simp at prop₁ prop₄
                                                     simp [Eq.symm prop₁] at prop₄)                                                                                  
     | ⟨x::xs, p₁⟩, ⟨y::ys, p₂⟩, ⟨z::zs, p₃⟩ => rw [Order.lex_impl]
                                                split
                                                simp
-                                               split
-                                               apply aux (m-1) (tail ⟨x::xs, p₁⟩) (tail ⟨y::ys, p₂⟩) (tail ⟨z::zs, p₃⟩)
-                                               rw [Order.lex_impl] at h
-                                               split at h
-                                               rename_i prop₁ _ _ _ _ _ _ prop₂ _ _
-                                               simp at prop₁ prop₂
-                                               simp [Eq.symm prop₂] at prop₁
-                                               split at h
-                                               exact h
-                                               simp at *
-                                               rename_i var_mul₁ var_mul₂ _ _ _ _ _ _ _ _ eq neq heq₁ heq₂
-                                               simp [map₂, Variables.mul, List.zipWith] at var_mul₁ var_mul₂
-                                               have eq₁ := heq₁.left 
-                                               have eq₂ := heq₂.left
-                                               cases var_mul₁
-                                               cases var_mul₂
-                                               rename_i sum_eq _
-                                               simp [eq₁, eq₂] at sum_eq
-                                               contradiction
-                                               rw [Order.lex_impl] at h
-                                               split at h
-                                               simp at *
-                                               split at h
-                                               rename_i var_mul₁ var_mul₂ _ _ _ _ _ _ _ _ _ heq₁ heq₂ eq
-                                               simp [map₂, Variables.mul, List.zipWith] at var_mul₁ var_mul₂
-                                               cases heq₁
-                                               cases heq₂
-                                               cases var_mul₁
-                                               cases var_mul₂
-                                               simp [eq]
-                                               rename_i eq _ _ hneq₂ _
-                                               simp at *
-                                               contradiction
-                                               rename_i var_mul₁ var_mul₂ _ _ _ _ _ _ _ _ _ heq₁ heq₂ neq
-                                               cases heq₁
-                                               cases heq₂
-                                               cases var_mul₁
-                                               cases var_mul₂
-                                               simp
-                                               exact h
+                                               sorry
+                                               sorry
+                                               --split
+                                               --apply aux (m-1) (tail ⟨x::xs, p₁⟩) (tail ⟨y::ys, p₂⟩) (tail ⟨z::zs, p₃⟩)
+                                               --rw [Order.lex_impl] at h
+                                               --split at h
+                                               --rename_i prop₁ _ _ _ _ _ _ prop₂ _ _
+                                               --simp at prop₁ prop₂
+                                               --simp [Eq.symm prop₂] at prop₁
+                                               --split at h
+                                               --exact h
+                                               --simp at *
+                                               --rename_i var_mul₁ var_mul₂ _ _ _ _ _ _ _ _ eq neq heq₁ heq₂
+                                               --simp [map₂, Variables.mul, List.zipWith] at var_mul₁ var_mul₂
+                                               --have eq₁ := heq₁.left 
+                                               --have eq₂ := heq₂.left
+                                               --cases var_mul₁
+                                               --cases var_mul₂
+                                               --rename_i sum_eq _
+                                               --simp [eq₁, eq₂] at sum_eq
+                                               --contradiction
+                                               --rw [Order.lex_impl] at h
+                                               --split at h
+                                               --simp at *
+                                               --split at h
+                                               --rename_i var_mul₁ var_mul₂ _ _ _ _ _ _ _ _ _ heq₁ heq₂ eq
+                                               --simp [map₂, Variables.mul, List.zipWith] at var_mul₁ var_mul₂
+                                               --cases heq₁
+                                               --cases heq₂
+                                               --cases var_mul₁
+                                               --cases var_mul₂
+                                               --simp [eq]
+                                               --rename_i eq _ _ hneq₂ _
+                                               --simp at *
+                                               --contradiction
+                                               --rename_i var_mul₁ var_mul₂ _ _ _ _ _ _ _ _ _ heq₁ heq₂ neq
+                                               --cases heq₁
+                                               --cases heq₂
+                                               --cases var_mul₁
+                                               --cases var_mul₂
+                                               --simp
+                                               --exact h
   apply aux n v₁ v₂ v₃
 
+--# Decidable theorems
 theorem lex_true_of_blt_lex_true (h: Eq (Order.blt_lex_impl v₁ v₂) true): Order.lex v₁ v₂ := by
   let rec aux (m: Nat) (a b: Vector Nat m) (h: Eq (Order.blt_lex_impl a b) true): Order.lex a b := by
     rw [Order.lex]
     rw [Order.lex_impl]
     match a, b with
-      | ⟨[], _⟩  , ⟨[], _⟩     => simp
+      | ⟨[], _⟩  , ⟨[], _⟩     => rw [Order.blt_lex_impl] at h
+                                  split at h
+                                  simp at *
+                                  split
+                                  rename_i heq _ _
+                                  simp at heq
+                                  rename_i heq _ _
+                                  simp at heq
       | ⟨x::xs, _⟩, ⟨y::ys, _⟩ => split
+                                  rw [Order.blt_lex_impl] at h
+                                  split at h
+                                  simp at h
+                                  rename_i heq₁ heq₂ _ _ _ _ _ _ _ _ heq₃ heq₄ 
+                                  split at h
+                                  rw [heq₁] at heq₃ 
+                                  rw [heq₂] at heq₄
+                                  rename_i heq
+                                  sorry
+                                  sorry
                                   simp
                                   split
                                   rw [Order.blt_lex_impl] at h
@@ -381,64 +404,54 @@ theorem lex_true_of_blt_lex_true (h: Eq (Order.blt_lex_impl v₁ v₂) true): Or
   rename_i n
   exact aux n v₁ v₂ h                                 
 
-theorem blt_eq_true_of_lex (h: Order.lex_impl v₁ v₂) : Eq (Order.blt_lex_impl v₁ v₂) true := by
-  let rec aux (m: Nat) (a b: Vector Nat m) (h: Order.lex_impl a b): Eq (Order.blt_lex_impl a b) true := by 
+theorem lex_le_true_of_blt_lex_true (h: Eq (Order.blt_lex_impl v₁ v₂) true): Order.lex_le v₁ v₂ := by 
+  rw [Order.lex_le]
+  split
+  simp
+  simp [lex_true_of_blt_lex_true, h]
+
+theorem blt_eq_true_of_lex_le (h: Order.lex_le v₁ v₂) : Eq (Order.ble_lex_impl v₁ v₂) true := by
+  let rec aux (m: Nat) (a b: Vector Nat m) (h: Order.lex_le a b): Eq (Order.ble_lex_impl a b) true := by 
      match a, b with
-      | ⟨[], _⟩, ⟨[], _⟩       => rw [Order.blt_lex_impl]
-      | ⟨x::xs, _⟩, ⟨y::ys, _⟩ => rw [Order.blt_lex_impl]
-                                  split;rfl
-                                  split
-                                  rw [Order.lex_impl] at h
-                                  simp at h
+      | ⟨[], _⟩, ⟨[], _⟩       => rw [Order.lex_le] at h
                                   split at h
-                                  apply blt_eq_true_of_lex h
-                                  rename_i heq₁ heq₂ neq eq
-                                  simp at heq₁ heq₂
-                                  have eq₁ := heq₁.left
-                                  have eq₂ := heq₂.left
-                                  simp at neq
-                                  rw [eq₁, eq₂] at eq
-                                  contradiction
-                                  rw [Order.lex_impl] at h
-                                  simp at h
-                                  split at h
-                                  rename_i heq₁ heq₂ neq eq
-                                  simp at heq₁ heq₂
-                                  have eq₁ := heq₁.left
-                                  have eq₂ := heq₂.left
-                                  simp at neq
-                                  rw [eq₁, eq₂] at eq
-                                  contradiction
+                                  rw [Order.ble_lex_impl]
                                   simp
-                                  rename_i heq₁ heq₂ _ _
-                                  simp at heq₁ heq₂
-                                  have eq₁ := Eq.symm heq₁.left
-                                  have eq₂ := Eq.symm heq₂.left
-                                  rwa [eq₁, eq₂]
+                                  simp at *
+      | ⟨x::xs, _⟩, ⟨y::ys, _⟩ => rw [Order.lex_le] at h
+                                  split at h
+                                  rw [Order.ble_lex_impl, algebra.Order.blt_lex_impl]
+                                  simp
+                                  rename_i heq 
+                                  split
+                                  simp [heq]
+                                  cases heq
+                                  simp
+                                  rw [Order.lex, Order.lex_impl] at h
+                                  rw [Order.ble_lex_impl, algebra.Order.blt_lex_impl]
+                                  split at h
+                                  simp at *
+                                  split at h
+                                  simp at *
+                                  simp
+                                  split
+                                  sorry
+                                  sorry
+                                  sorry
   rename_i n
   exact aux n v₁ v₂ h 
 
-theorem lex_false_of_blt_lex_false (h: Not (Eq (Order.blt_lex_impl v₁ v₂) true)): Not (Order.lex v₁ v₂) :=
-  fun h' => absurd (blt_eq_true_of_lex h') h
-
-instance Order.lex_decidable (v₁ v₂: Variables n order.Lex): Decidable (Order.lex v₁ v₂) :=
-  dite (Eq (Order.blt_lex_impl v₁ v₂) true) (fun h => isTrue (lex_true_of_blt_lex_true h))
-                                            (fun h => isFalse (lex_false_of_blt_lex_false h))
-
-end monomials_lex_order
+theorem lex_le_false_of_blt_lex_false (h: Not (Eq (Order.ble_lex_impl v₁ v₂) true)): Not (Order.lex_le v₁ v₂) :=  
+  fun h' => absurd (blt_eq_true_of_lex_le h') h
 
 
-section monomials_grlex_order
+instance Order.lex_decidable (v₁ v₂: Variables n order.Lex): Decidable (Order.lex_le v₁ v₂) :=
+  dite (Eq (Order.blt_lex_impl v₁ v₂) true) (fun h => isTrue (lex_le_true_of_blt_lex_true h))
+                                            (fun h => isFalse (lex_le_false_of_blt_lex_false h))
 
-private def Order.bgrlex (vs₁ vs₂: Variables n order.GrLex): Bool :=
-  let sum₁ := elem_sum vs₁ 
-  let sum₂ := elem_sum vs₂   
-  if sum₁ < sum₂ then true
-  else if sum₁ = sum₂ then Order.lex vs₁ vs₂
-  else false
-  where
-    elem_sum (vs: Variables n order.GrLex): Nat :=
-      List.foldl (fun x y => x + y) 0 vs.toList
+
+--# Grlex order
+--# a <_grlex b ↔ |a| < |b| ∨ |a| = |b| ∧ a <_lex b 
 
 def Order.grlex (vs₁ vs₂: Variables n order.GrLex): Prop :=
   let sum₁ := elem_sum vs₁ 
@@ -450,8 +463,19 @@ def Order.grlex (vs₁ vs₂: Variables n order.GrLex): Prop :=
     elem_sum (vs: Variables n order.GrLex): Nat :=
       List.foldl (fun x y => x + y) 0 vs.toList
 
-def Order.grlex_le (v₁ v₂ : Variables n order.GrLex): Prop := v₁ = v₂ ∨ Order.grlex v₁ v₂  
+def Order.grlex_le (v₁ v₂ : Variables n order.GrLex): Prop := v₁ = v₂ ∨ Order.grlex v₁ v₂ 
 
+private def Order.bgrlex (vs₁ vs₂: Variables n order.GrLex): Bool :=
+  let sum₁ := elem_sum vs₁ 
+  let sum₂ := elem_sum vs₂   
+  if sum₁ < sum₂ then true
+  else if sum₁ = sum₂ then Order.blt_lex_impl vs₁ vs₂
+  else false
+  where
+    elem_sum (vs: Variables n order.GrLex): Nat :=
+      List.foldl (fun x y => x + y) 0 vs.toList 
+
+--# Ordering theorems
 theorem grlex_lt_iff_le_not_le : ∀ (a b : Variables n order.GrLex), Order.grlex a b ↔ Order.grlex_le a b ∧ ¬Order.grlex_le b a := 
   by 
     intros a b 
@@ -462,7 +486,7 @@ theorem grlex_lt_iff_le_not_le : ∀ (a b : Variables n order.GrLex), Order.grle
 theorem grlex_lt_refl: ∀ (a : Variables n order.GrLex), Order.grlex a a := by 
   intros a
   simp [Order.grlex]
-  apply lex_lt_refl
+  sorry
 
 theorem grlex_le_refl: ∀ (a : Variables n order.GrLex), Order.grlex_le a a := by
   intros a
@@ -585,7 +609,7 @@ theorem grlex_lt_total : ∀ (a b : Variables n order.GrLex), Order.grlex a b �
   simp [Order.grlex]
   split <;> simp
   split <;> repeat (first | split | simp)
-  simp [lex_lt_total] 
+  sorry
   rename_i nleq₁ eq nleq₂ neq
   have contr := Eq.symm eq 
   contradiction
@@ -604,6 +628,16 @@ theorem grlex_le_total : ∀ (a b : Variables n order.GrLex), Order.grlex_le a b
   rw [or_or_or_comm]
   simp [grlex_lt_total]
 
+theorem grlex_add_lt_add : ∀ a b c: Variables n order.GrLex, Order.grlex a b → Order.grlex (Variables.mul a c) (Variables.mul b c) := by
+  intros v₁ v₂ v₃
+  let rec aux (m: Nat) (a b c: Variables m order.GrLex) : Order.grlex a b → Order.grlex (Variables.mul a c) (Variables.mul b c) := by
+    intros h 
+    match a, b, c with
+      | ⟨[], _⟩, ⟨[], _⟩, ⟨[], _⟩          => sorry
+      | ⟨x::xs, p₁⟩, ⟨y::ys, p₂⟩, ⟨z::zs, p₃⟩ => sorry
+  exact aux n v₁ v₂ v₃ 
+
+--# Decidable theorems
 theorem grlex_true_of_blt_grlex_true (h: Eq (Order.bgrlex v₁ v₂) true): Order.grlex v₁ v₂ := by
   simp [Order.grlex]
   split
@@ -659,19 +693,8 @@ theorem grblt_eq_true_of_grlex (h: Order.grlex v₁ v₂): Eq (Order.bgrlex v₁
 theorem grlex_false_of_blt_grlex_false (h: Not (Eq (Order.bgrlex v₁ v₂) true)): Not (Order.grlex v₁ v₂) := 
   fun h' => absurd (grblt_eq_true_of_grlex h') h
   
-instance Order.grlex_decidable (v₁ v₂: Variables n order.GrLex): Decidable (Order.grlex v₁ v₂) := 
+instance grlex_decidable (v₁ v₂: Variables n order.GrLex): Decidable (Order.grlex v₁ v₂) := 
   dite (Eq (Order.bgrlex v₁ v₂) true) (fun h => isTrue (grlex_true_of_blt_grlex_true h))
                                       (fun h => isFalse (grlex_false_of_blt_grlex_false h))
-
-theorem grlex_add_lt_add : ∀ a b c: Variables n order.GrLex, Order.grlex a b → Order.grlex (Variables.mul a c) (Variables.mul b c) := by
-  intros v₁ v₂ v₃
-  let rec aux (m: Nat) (a b c: Variables m order.GrLex) : Order.grlex a b → Order.grlex (Variables.mul a c) (Variables.mul b c) := by
-    intros h 
-    match a, b, c with
-      | ⟨[], _⟩, ⟨[], _⟩, ⟨[], _⟩          => sorry
-      | ⟨x::xs, p₁⟩, ⟨y::ys, p₂⟩, ⟨z::zs, p₃⟩ => sorry
-  exact aux n v₁ v₂ v₃ 
-
-end monomials_grlex_order
 
 end algebra
